src/Lean/Meta/Tactic/Cbv/CbvProc.lean
@@ -1,0 +1,71 @@
+module
+
+prelude
+public import Lean.Meta.Tactic.Cbv.Types
+public import Lean.Elab.Term.TermElabM
+public import Lean.Compiler.IR
+public meta import Lean.Meta.Tactic.Cbv.Types
+public section
+
+namespace Lean.Meta.Tactic.Cbv
+
+open Lean.Elab
+open Lean.Elab.Term
+
+def mkNormNumExt (n : Name) : ImportM CbvExt := do
+  let { env, opts, .. } ← read
+  IO.ofExcept <| unsafe env.evalConstCheck CbvExt opts ``CbvExt n
+
+initialize cbvExt : ScopedEnvExtension Entry (Entry × CbvExt) CbvExtState ←
+  -- we only need this to deduplicate entries in the DiscrTree
+  have : BEq CbvExt := ⟨fun _ _ ↦ false⟩
+  /- Insert `v : NormNumExt` into the tree `dt` on all key sequences given in `kss`. -/
+  let insert kss v dt := kss.foldl (fun dt ks ↦ dt.insertKeyValue ks v) dt.1
+  registerScopedEnvExtension {
+    mkInitial := pure {}
+    ofOLeanEntry := fun _ e@(_, n) ↦ return (e, ← mkNormNumExt n)
+    toOLeanEntry := (·.1)
+    addEntry := fun { tree } ((kss, n), ext) ↦
+      { tree := insert kss ext tree }
+  }
+
+syntax (name := cbv_proc) "cbv_proc " term,+ : attr
+
+initialize registerBuiltinAttribute {
+  name := `cbv_proc
+  descr := "adds a norm_num extension"
+  applicationTime := .afterCompilation
+  add := fun declName stx kind ↦ match stx with
+  | `(attr| cbv_proc $es,*) => do
+    let env ← getEnv
+    ensureAttrDeclIsMeta `cbv_proc declName kind
+    unless (env.getModuleIdxFor? declName).isNone do
+      throwError "invalid attribute 'norm_num', declaration is in an imported module"
+    if (IR.getSorryDep env declName).isSome then return -- ignore in progress definitions
+    let ext ← mkNormNumExt declName
+    let keys ← MetaM.run' <| es.getElems.mapM fun stx ↦ do
+      let e ← TermElabM.run' <| withSaveInfoContext <| withAutoBoundImplicit <|
+        withReader ({ · with ignoreTCFailures := true }) do
+          let e ← elabTerm stx none
+          let (_, _, e) ← lambdaMetaTelescope (← mkLambdaFVars (← getLCtx).getFVars e)
+          return e
+      DiscrTree.mkPath e
+    cbvExt.add ((keys, declName), ext) kind
+    -- TODO: track what `[cbv_proc]` decls are actually used at use sites
+    recordExtraRevUseOfCurrentModule
+  | _ => throwUnsupportedSyntax
+  erase := fun declName => do throwError "not implemented: erasing"
+}
+
+def runCbvProcs (e : Expr) (callback : Expr → CbvM Result): CbvM <| Option Result := do
+  let cbvProcs := cbvExt.getState (← getEnv)
+  let arr ← cbvProcs.tree.getMatch e
+  let mut res : Option Result := .none
+  for ext in arr do
+    let evalResult ← ext.eval e callback
+    if (evalResult.isSome) then
+      res := evalResult
+      break
+  return res
+
+end Lean.Meta.Tactic.Cbv
