src/Lean/Meta/Tactic/Cbv/Types.lean
@@ -8,8 +8,9 @@ module
 prelude
 public import Lean.Expr
 public import Lean.Meta.Basic
-public import Lean.Data.PersistentHashMap
+public import Std.Data.HashMap
 public import Lean.Meta.CongrTheorems
+public import Lean.Meta.DiscrTree
 public section
 
 namespace Lean.Meta.Tactic.Cbv
@@ -25,9 +26,45 @@ structure Key where
 deriving BEq, Hashable
 
 structure CbvState where
-  compositionThms : PersistentHashMap Key CongrTheorem
-  leftCongruenceThms : PersistentHashMap Key Expr
+  compositionThms : Std.HashMap Key CongrTheorem
+  leftCongruenceThms : Std.HashMap Key Expr
+  fullyEvaluated : Std.HashSet Expr
 
 abbrev CbvM := StateT CbvState MetaM
+
+abbrev CbvProc := (e : Expr) → (callback : Expr → CbvM Result) → CbvM (Option Result)
+
+structure ExtensionState where
+  tree : DiscrTree CbvProc := {}
+  deriving Inhabited
+
+structure CbvExt where
+  /-- Attempts to prove an expression is equal to some explicit vale the relevant type. -/
+  eval : CbvProc
+  /-- The name of the `cbv` extension. -/
+  name : Name := by exact decl_name%
+
+/-- The state of the `cbv` extension environment -/
+structure CbvExtState where
+  /-- The tree of `cbv` extensions. -/
+  tree : DiscrTree CbvExt := {}
+  deriving Inhabited
+
+inductive CbvCongrArgKind where
+  -- Requires the proof that it evaluates to a value
+  | eval
+  -- It is a value, no need to pass the proof
+  | value
+  -- Needs to be finished off with refl
+  | refl
+  deriving Inhabited, Repr, BEq
+
+instance : ToMessageData CbvCongrArgKind where
+  toMessageData := fun a => match a with
+  | .eval => "eval"
+  | .refl => "refl"
+  | .value => "value"
+
+abbrev Entry := Array (Array DiscrTree.Key) × Name
 
 end Lean.Meta.Tactic.Cbv
